% func-image.tex

%%%%%%%%%%%%%%%
\begin{frame}{}
  \begin{definition}[Restriction]
    The \red{\it restriction} of a function $f: A \to B$ to $X$
    is the \blue{function}:

    \[
      f|_{X} = \set{(x, y) \in f \mid \purple{x \in X}}
    \]
  \end{definition}

  \pause
  \[
    \text{It is \cyan{unnecessary} that } X \subseteq A,\;
    \text{though it is \cyan{usually} the case.}
  \]

  \pause
  \[
    f|_{X}: \purple{A \cap X} \to B
  \]

  \[
    \forall x \in A \cap X.\; f|_{X}(x) = f(x)
  \]
\end{frame}
%%%%%%%%%%%%%%%

%%%%%%%%%%%%%%%
\begin{frame}{}
  \begin{definition}[像 (Image)]
    The \red{\it image} of $X$ under a function $f: A \to B$ is the set
    \[
      {f(X) = \set{y \mid \exists \purple{x \in X}.\; (x, y) \in f}}
    \]
  \end{definition}

  \pause
  \[
    \text{It is \teal{unnecessary} that } X \subseteq \dom(f) = A,
    \text{though it is \teal{usually} the case.}
  \]

  \pause
  \[
    f(X) = f(\purple{A \cap X})
  \]

  \pause
  \[
    f(\set{a}) = \set{b} \quad \text{简记为} \quad f(a) = b
  \]
\end{frame}
%%%%%%%%%%%%%%%

%%%%%%%%%%%%%%%
\begin{frame}{}
  \begin{definition}[像 (Image)]
    The \red{\it image} of $X$ under a function $f: A \to B$ is the set
    \[
      {f(X) = \set{y \mid \exists \purple{x \in X}.\; (x, y) \in f}}
    \]
  \end{definition}

  \vspace{0.30cm}
  \[
    \red{\boxed{y \in f(X) \iff \exists x \in X.\; y = f(x)}}
  \]
\end{frame}
%%%%%%%%%%%%%%%

%%%%%%%%%%%%%%%
\begin{frame}{}
  \begin{definition}[逆像 (Inverse Image)]
    The \red{\it inverse image} of $Y$ under a function $f: A \to B$ is the set
    \[
      {f^{-1}(Y) = \set{x \mid \exists \purple{y \in Y}.\; (x, y) \in f}}
    \]
  \end{definition}

  \pause
  \[
    \text{It is \teal{unnecessary} that } Y \subseteq \ran(f),
    \text{though it is \teal{usually} the case.}
  \]

  \pause
  \[
    f^{-1}(Y) = f^{-1}(\purple{Y \cap \ran(f)})
  \]

  \pause
  \[
    f^{-1}(\set{b}) = \set{a}
      \quad\text{\blue{可简记为}}\quad f^{-1}(b) = \set{a}
      \quad\text{\red{不能简记为}}\quad f^{-1}(b) = a
  \]
\end{frame}
%%%%%%%%%%%%%%%

%%%%%%%%%%%%%%%
\begin{frame}{}
  \begin{definition}[逆像 (Inverse Image)]
    The \red{\it inverse image} of $Y$ under a function $f: A \to B$ is the set
    \[
      {f^{-1}(Y) = \set{x \mid \exists \purple{y \in Y}.\; (x, y) \in f}}
    \]
  \end{definition}

  \vspace{0.30cm}
  \[
    \red{\boxed{x \in f^{-1}(Y) \iff f(x) \in Y}}
  \]
\end{frame}
%%%%%%%%%%%%%%%

%%%%%%%%%%%%%%%
\begin{frame}{}
  \[
    \red{\boxed{y \in f(X) \iff \exists x \in X.\; y = f(x)}}
  \]

  \[
    \red{\boxed{x \in f^{-1}(Y) \iff f(x) \in Y}}
  \]
\end{frame}
%%%%%%%%%%%%%%%

%%%%%%%%%%%%%%%
\begin{frame}{}
  \[
    f: A \to B
  \]

  \[
    a \in A_{0} \red{\;\centernot\implies\;} f(a) \in f(A_{0})
  \]

  \pause
  \[
    a \in A_{0} \purple{\;\cap\; A} \blue{\;\implies\;} f(a) \in f(A_{0})
  \]
\end{frame}
%%%%%%%%%%%%%%%

%%%%%%%%%%%%%%%
\begin{frame}{}
  \begin{theorem}[Properties of $f$ and $f^{-1}$]
    \[
      f: A \to B \qquad
      \xout{A_1, A_2 \subseteq A,\; B_1, B_2 \subseteq B}
    \]

    \begin{enumerate}[(i)]
      \item \purple{$f$ preserves only $\subseteq$ and $\cup$:}
        \begin{enumerate}[(1)]
          \setlength{\itemsep}{8pt}
          \item $A_1 \subseteq A_2 \implies f(A_1) \subseteq f(A_2)$
          \item \teal{$f(A_1 \cup A_2) = f(A_1) \cup f(A_2)$}
          \item $f(A_1 \cap A_2) \subseteq f(A_1) \cap f(A_2)$
          \item $f(A_1 \setminus A_2) \supseteq f(A_1) \setminus f(A_2)$
        \end{enumerate}
    \end{enumerate}
  \end{theorem}
\end{frame}
%%%%%%%%%%%%%%%

%%%%%%%%%%%%%%%
\begin{frame}{}
  \begin{theorem}
    \[
      f: A \to B
    \]
    \[
      A_1 \subseteq A_2 \implies f(A_1) \subseteq f(A_2)
    \]
  \end{theorem}

  \pause
  \vspace{0.30cm}
  \red{对任意 $b$,}
  \setcounter{equation}{0}
  \begin{align}
    &b \in f(A_{1}) \\[6pt]
    \uncover<3->{\iff & \exists a \in A_{1}.\; b = f(a) \\[6pt]}
    \uncover<4->{\red{\implies} & \exists a \in A_{2}.\; b = f(a) \\[6pt]}
    \uncover<5->{\iff & b \in f(A_{2})}
  \end{align}
\end{frame}
%%%%%%%%%%%%%%%

%%%%%%%%%%%%%%%
\begin{frame}{}
  \begin{theorem}
    \[
      f: A \to B
    \]
    \[
      f(A_1 \cap A_2) \red{\;\subseteq\;} f(A_1) \cap f(A_2)
    \]
  \end{theorem}

  \pause
  \vspace{0.30cm}
  \red{对任意 $b$,}
  \setcounter{equation}{0}
  \begin{align}
    &b \in f(A_1 \cap A_2) \\[6pt]
    \onslide<3->{\iff & \exists a \in A_1 \cap A_2.\; b = f(a) \\[6pt]}
    \onslide<4->{\red{\implies}& \big(\exists a \in A_{1}.\; b = f(a)\big)
      \land \big(\exists a \in A_{2}.\; b = f(a)\big) \\[6pt]}
    \onslide<5->{\iff & b \in f(A_{1}) \land b = f(A_{2}) \\[6pt]}
    \onslide<6->{\iff & b \in f(A_1) \cap f(A_2)}
  \end{align}

  \begin{center}
    \onslide<7->{\red{$Q:$ When does $f(A_1 \cap A_2) \red{\;=\;} f(A_1) \cap f(A_2)$ hold?} \\[5pt]}
    \onslide<8->{\teal{$f$ is injective.}}
  \end{center}
\end{frame}
%%%%%%%%%%%%%%%

%%%%%%%%%%%%%%%
\begin{frame}{}
  \begin{theorem}
    \[
      f: A \to B
    \]
    \[
      f(A_1 \setminus A_2) \red{\;\supseteq\;} f(A_1) \setminus f(A_2)
    \]
  \end{theorem}

  \pause
  \vspace{0.30cm}
  \red{对任意 $b$,}
  \setcounter{equation}{0}
  \begin{align}
    &b \in f(A_{1}) \setminus f(A_{2}) \\[6pt]
    \uncover<3->{\iff & b \in f(A_{1}) \land b \notin f(A_{2}) \\[6pt]}
    \uncover<4->{\iff & (\exists a_{1} \in A_{1}.\; b = f(a_{1})) \land
      (\forall a_{2} \in A_{2}.\; b \neq f(a_{2})) \\[6pt]}
    \uncover<6->{\red{\implies} & \exists a \in A_{1} \setminus A_{2}.\; b = f(a) \\[6pt]}
    \uncover<5->{\iff & b \in f(A_{1} \setminus A_{2})}
  \end{align}
\end{frame}
%%%%%%%%%%%%%%%

%%%%%%%%%%%%%%%
\begin{frame}{}
  \begin{theorem}[Properties of $f$ and $f^{-1}$]
    \[
      f: A \to B \qquad
      \xout{A_1, A_2 \subseteq A,\; B_1, B_2 \subseteq B}
    \]

    \begin{enumerate}[(i)]
      \setcounter{enumi}{1}
      \item \purple{$f^{-1}$ preserves $\subseteq$, $\cup$, $\cap$, and $\setminus$:}
        \begin{enumerate}[(1)]
          \setlength{\itemsep}{8pt}
          \setcounter{enumii}{4}
          \item $B_1 \subseteq B_2 \implies f^{-1}(B_1) \subseteq f^{-1}(B_2)$
          \item \teal{$f^{-1}(B_1 \cup B_2) = f^{-1}(B_1) \cup f^{-1}(B_2)$}
          \item $f^{-1}(B_1 \cap B_2) = f^{-1}(B_1) \cap f^{-1}(B_2)$
          \item \teal{$f^{-1}(B_1 \setminus B_2) = f^{-1}(B_1) \setminus f^{-1}(B_2)$}
        \end{enumerate}
    \end{enumerate}
  \end{theorem}
\end{frame}
%%%%%%%%%%%%%%%

%%%%%%%%%%%%%%%
\begin{frame}{}
  \begin{theorem}
    \[
      f: A \to B
    \]
    \[
      B_1 \subseteq B_2 \implies f^{-1}(B_1) \subseteq f^{-1}(B_2)
    \]
  \end{theorem}

  \pause
  \vspace{0.30cm}
  \red{对任意 $a$,}
  \setcounter{equation}{0}
  \begin{align}
    &a \in f^{-1}(B_{1}) \\[6pt]
    \uncover<3->{\iff & f(a) \in B_{1} \\[6pt]}
    \uncover<4->{\red{\implies} & f(a) \in B_{2} \\[6pt]}
    \uncover<5->{\iff & a \in f^{-1}(B_{2})}
  \end{align}
\end{frame}
%%%%%%%%%%%%%%%

%%%%%%%%%%%%%%%
\begin{frame}{}
  \begin{theorem}
    \[
      f: A \to B
    \]
    \[
      f^{-1}(B_1 \cap B_2) = f^{-1}(B_1) \cap f^{-1}(B_2)
    \]
  \end{theorem}

  \pause
  \vspace{0.30cm}
  \red{对任意 $a$,}
  \setcounter{equation}{0}
  \begin{align}
    &a \in f^{-1}(B_{1} \cap B_{2}) \\[6pt]
    \uncover<3->{\iff & f(a) \in B_{1} \cap B_{2} \\[6pt]}
    \uncover<4->{\iff & f(a) \in B_{1} \land f(a) \in B_{2} \\[6pt]}
    \uncover<5->{\iff & a \in f^{-1}(B_{1}) \land a \in f^{-1}(B_{2}) \\[6pt]}
    \uncover<6->{\iff & a \in f^{-1}(B_{1}) \cap f^{-1}(B_{2})}
  \end{align}
\end{frame}
%%%%%%%%%%%%%%%

%%%%%%%%%%%%%%%
\begin{frame}{}
  \begin{theorem}[Properties of $f$ and $f^{-1}$]
    \[
      f: A \to B
    \]

    \begin{enumerate}[(i)]
      \setcounter{enumi}{2}
      \item $f$ and $f^{-1}$: \\[8pt]
        \begin{enumerate}[(1)]
          \setlength{\itemsep}{10pt}
          \setcounter{enumii}{8}
            \item $\purple{A_0 \subseteq A} \implies A_0 \subseteq f^{-1}(f(A_0))$
            \item \teal{$B_0 \supseteq f(f^{-1}(B_0))$}
        \end{enumerate}
    \end{enumerate}
  \end{theorem}
\end{frame}
%%%%%%%%%%%%%%%

%%%%%%%%%%%%%%%
\begin{frame}{}
  \begin{theorem}
    \[
      f: A \to B
    \]
    \[
      A_0 \subseteq A \implies A_0 \subseteq f^{-1}(f(A_0))
    \]
  \end{theorem}

  \pause
  \vspace{0.30cm}
  \red{对任意 $b$,}
  \setcounter{equation}{0}
  \begin{align}
    &a \in A_{0} \\[6pt]
    \uncover<3->{\implies & a \in A_{0} \purple{\;\cap\; A} \\[6pt]}
    \uncover<4->{\red{\implies} & f(a) \in f(A_{0}) \\[6pt]}
    \uncover<5->{\iff & a \in f^{-1}(f(A_{0}))}
  \end{align}
\end{frame}
%%%%%%%%%%%%%%%

%%%%%%%%%%%%%%%
% \begin{frame}{}
%   \begin{theorem}[]
%     \[
%       f: A \to B
%     \]
%     \[
%       B_0 \supseteq f(f^{-1}(B_0))
%     \]
%   \end{theorem}
%
%   \pause
%   \vspace{0.30cm}
%   \red{对任意 $b$,}
%   \setcounter{equation}{0}
%   \begin{align}
%     &b \in f(f^{-1}(B_0)) \\[6pt]
%     \onslide<3->{\iff & \exists a \in f^{-1}(B_0).\; b = f(a) \\[6pt]}
%     \onslide<4->{\iff & \exists a \in A.\; f(a) \in B_0 \land b = f(a) \\[6pt]}
%     \onslide<5->{\red{\implies} & b \in B_0}
%   \end{align}
% 
%   \begin{center}
%     \onslide<6->{\red{$Q$: When does $B_0 = f(f^{-1}(B_0))$ hold?} \\[8pt]}
%     \onslide<7->{\teal{$f$ is surjective and $B_0 \subseteq \ran(f)$.}}
%   \end{center}
% \end{frame}
%%%%%%%%%%%%%%%