% prop-logic-inference.tex

%%%%%%%%%%%%%%%%%%%%
\begin{frame}{}
  \begin{center}
    {\Large 命题逻辑的自然推理 (演绎; 推演) 系统}
  \end{center}
\end{frame}
%%%%%%%%%%%%%%%%%%%%

%%%%%%%%%%%%%%%%%%%%
\begin{frame}{}
  \begin{center}
    从上往下看
    \[
      \nd{\alpha \quad\text{(前提)}}{\beta \quad\text{(结论)}}{\text{规则名称}}
    \]
    从下往上看
  \end{center}
\end{frame}
%%%%%%%%%%%%%%%%%%%%

%%%%%%%%%%%%%%%%%%%%
\begin{frame}{}
  \[
    \nd{}{P}{\text{unit}} \qquad P \text{ is an axiom} ???
  \]
\end{frame}
%%%%%%%%%%%%%%%%%%%%

%%%%%%%%%%%%%%%%%%%%
\begin{frame}
  \[
    \nd{}{[x : P]}{\text{assum}}
  \]

  \vspace{0.50cm}
  \begin{center}
    所有新引入的假设最终必须被``\red{\bf 释放}''(discharged)
  \end{center}
\end{frame}
%%%%%%%%%%%%%%%%%%%%

%%%%%%%%%%%%%%%%%%%%
\begin{frame}{}
  \begin{gather*}
    \nd{\stackrel{[x \;:\; P]}{\stackrel{\vdots}{Q}}}{P \to Q}{\to\text{-intro}/x} \\[10pt]
    \text{\blue{Assumption $x$ is discharged}} \\[35pt]
    \nd{P \qquad P \to Q}{Q}{\to\text{-elim, modus ponens}}
  \end{gather*}
\end{frame}
%%%%%%%%%%%%%%%%%%%%

%%%%%%%%%%%%%%%%%%%%
\begin{frame}{}
  \begin{gather*}
    \nd{P \qquad Q}{P \land Q}{\land\text{-intro}} \\[35pt]
    \nd{P \land Q}{P}{\land\text{-elim-left}} \\[35pt]
    \nd{P \land Q}{Q}{\land\text{-elim-right}}
  \end{gather*}
\end{frame}
%%%%%%%%%%%%%%%%%%%%

%%%%%%%%%%%%%%%%%%%%
\begin{frame}{}
  \begin{gather*}
    \nd{P}{P \lor Q}{\lor\text{-intro-left}} \\[35pt]
    \nd{Q}{P \lor Q}{\lor\text{-intro-right}} \\[35pt]
    \nd{P \lor Q \qquad P \to R \qquad Q \to R}{R}{\lor\text{-elim}} \\[35pt]
  \end{gather*}
\end{frame}
%%%%%%%%%%%%%%%%%%%%

%%%%%%%%%%%%%%%%%%%%
\begin{frame}{}
  \begin{gather*}
    \nd{P \to \bot}{\lnot P}{\lnot\text{-intro}} \\[35pt]
    \nd{\lnot P}{P \to \bot}{\lnot\text{-elim}}
  \end{gather*}
\end{frame}
%%%%%%%%%%%%%%%%%%%%

%%%%%%%%%%%%%%%%%%%%
\begin{frame}{}
  \begin{gather*}
    \nd{\stackrel{[x \;:\; \lnot P]}{\stackrel{\vdots}{\bot}}}{P}{
      \text{RAA}/x \text{, reductio ad absurdum}} \\[35pt]
    \nd{\bot}{P}{\text{EFQ, ex falso quodlibet}}
  \end{gather*}
\end{frame}
%%%%%%%%%%%%%%%%%%%%

%%%%%%%%%%%%%%%%%%%%
\begin{frame}{}
  \[
    (A \to (B \to C)) \to ((A \land B) \to C)
  \]

  \pause
  \fig{width = 0.85\textwidth}{figs/chain-implication-proof}
\end{frame}
%%%%%%%%%%%%%%%%%%%%

%%%%%%%%%%%%%%%%%%%%
\begin{frame}{}
  \fig{width = 0.20\textwidth}{figs/chain-implication-proof-tree}
\end{frame}
%%%%%%%%%%%%%%%%%%%%